pulse/src/checker/Pulse.Checker.Abs.fst
@@ -68,8 +68,8 @@ let rec arrow_of_abs (env:_) (prog:st_term { Tm_Abs? prog.term })
         let arr, body = arrow_of_abs env body in
         let arr = close_term arr x in
         let body = close_st_term body x in
-        let ty : term = tm_fstar (tm_arrow b q (C_Tot arr))
-                                 (RU.union_ranges (RU.range_of_term b.binder_ty) (RU.range_of_term arr)) in
+        let ty : term = wr (tm_arrow b q (C_Tot arr))
+                           (RU.union_ranges (RU.range_of_term b.binder_ty) (RU.range_of_term arr)) in
         let prog : st_term = { prog with term = Tm_Abs { b; q; ascription; body}} in
         ty, prog
 
@@ -81,8 +81,8 @@ let rec arrow_of_abs (env:_) (prog:st_term { Tm_Abs? prog.term })
           //retain the original annotation, so that we check it wrt the inferred type in maybe_rewrite_body_typing
           let t = close_term t x in
           let annot = close_comp c x in
-          let ty : term = tm_fstar (tm_arrow b q (C_Tot t))
-                                   (RU.union_ranges (RU.range_of_term b.binder_ty) (RU.range_of_term t)) in
+          let ty : term = wr (tm_arrow b q (C_Tot t))
+                             (RU.union_ranges (RU.range_of_term b.binder_ty) (RU.range_of_term t)) in
           let ascription = { annotated = Some annot; elaborated = None } in
           let body = close_st_term body x in
           let prog : st_term = { prog with term = Tm_Abs { b; q; ascription; body} } in
@@ -103,7 +103,7 @@ let rec arrow_of_abs (env:_) (prog:st_term { Tm_Abs? prog.term })
         Env.fail env (Some prog.range) "Unannotated function body"
       
       | Some c -> ( //we're taking the annotation as is; remove it from the abstraction to avoid rechecking it
-        let ty : term = tm_fstar (tm_arrow b q c)
+        let ty : term = wr (tm_arrow b q c)
                                  (RU.union_ranges (RU.range_of_term b.binder_ty) (range_of_comp c)) in
         let ascription = empty_ascription in
         let body = close_st_term body x in
