pulse/src/checker/Pulse.Checker.Match.fst
@@ -48,7 +48,7 @@ let rec readback_pat (p : R.pattern) : option pattern =
     then None
     else
       let t = RU.deep_compress t in
-      let t = tm_fstar t Range.range_0 in
+      let t = wr t Range.range_0 in
       Some (Pat_Dot_Term (Some t))
 
   | _ -> None
@@ -245,7 +245,7 @@ let check_branch
   if (R.Tv_Unknown? (R.inspect_ln (fst (Some?.v elab_p)))) then
     fail g (Some e.range) "should not happen: pattern elaborated to Tv_Unknown";
   // T.print ("Elaborated pattern = " ^ T.term_to_string (fst (Some?.v elab_p)));
-  let eq_typ = mk_sq_eq2 sc_u sc_ty sc (tm_fstar (fst (Some?.v elab_p)) Range.range_0) in
+  let eq_typ = mk_sq_eq2 sc_u sc_ty sc (wr (fst (Some?.v elab_p)) Range.range_0) in
   let g' = push_binding g' hyp_var ({name = Sealed.seal "branch equality"; range = Range.range_0 }) eq_typ in
   let e = open_st_term_bs e pulse_bs in
   let pre_typing = tot_typing_weakening_n pulse_bs pre_typing in // weaken w/ binders
