pulse/src/checker/Pulse.Readback.fsti
@@ -20,35 +20,5 @@ module L = FStar.List.Tot
 open Pulse.Syntax.Base
 open Pulse.Elaborate.Pure
 
-val readback_qual (q:R.aqualv)
-  : option qualifier
-
-let is_view_of (tv:term_view) (t:term) : prop =
-  match tv with
-  | Tm_Emp -> t == tm_emp
-  | Tm_VProp -> t == tm_vprop
-  | Tm_Inames -> t == tm_inames
-  | Tm_EmpInames -> t == tm_emp_inames
-  | Tm_Star t1 t2 ->
-    t == tm_star t1 t2 /\
-    t1 << t /\ t2 << t
-  | Tm_ExistsSL u b body ->
-    t == tm_exists_sl u b body /\
-    u << t /\ b << t /\ body << t
-  | Tm_ForallSL u b body ->
-    t == tm_forall_sl u b body /\
-    u << t /\ b << t /\ body << t
-  | Tm_Pure p ->
-    t == tm_pure p /\
-    p << t
-  | Tm_Inv p ->
-    t == tm_inv p /\
-    p << t
-  | Tm_Unknown -> t == tm_unknown
-  | Tm_AddInv i is -> True
-
-val readback_ty (t:R.term)
-  : (r:option term_view { Some? r ==> Some?.v r `is_view_of` t })
-
 val readback_comp (t:R.term)
   : option (c:comp{ elab_comp c == t})
